\chapter{SOFR hedges}

\section{Hedging 3-month arithmetic with 3-month geometric}
Consider the case where we want to hedge: 
$$
X^{3M\_A} = \frac{1}{T-S}\int_{S}^{T}r_{u}du
$$

Here $[S,T]$ will denote a 3-month period, in the market we only have available
3-month futures $f^{3M}(t,S,T)$ (\ref{def: 3M_SOFR_futures})  calculated using a geometric average, this means that our hedge will look like: 
\begin{align*}
\argmin\limits_{a \in \R}\E_{Q}\left[
\left(
X^{3M\_A}-af^{3M}(t,S,T)
\right)^{2}
\bigg{|}\F_{t}
\right]
\end{align*}

Let's denote $H(a) :=\E_{Q}\left[
\left(X^{3M\_A}-af^{3M}(t,S,T)
\right)^{2}
\bigg{|}\F_{t}
\right]
$ 
expanding the square yields:
\begin{align*}
H(a) &= \E_{Q}\left[(X^{3M\_A})^{2}|\F_{t}\right] -2af^{3M}(t,S,T) +
a^{2}[f^{3M}(t,S,T)]^{2}
\end{align*}
Taking the derivative w.r.t. $a$ yields: 
\begin{align*}
H'(a) &= -2f^{3M}(t,S,T) + 2a[f^{3M}(t,S,T)]^{2}  
\end{align*} 

Now as $H''(a) = 2[f^{3M}(t,S,T)]^{2} > 0$, we have that the minimum is obtained by setting $H'(a) = 0$:
\begin{align*}
H'(a) &= 0 \\ 
&\Downarrow \\ 
a &= \frac{
\E_{Q}[X^{3M\_A}|\F_{t}]
}{
f^{3M}(t,S,T)
} \\ 
&= \frac{
\int_{S}^{T}\E_{Q}[r(u)|\F_{t}]du
}{
(T-S)f^{3M}(t,S,T)
}
\end{align*}

\begin{result}
Considering the above situation, we then have the following:
\begin{align*}
\argmin\limits_{a \in \R}\E_{Q}\left[
\left(
X^{3M\_A}-af^{3M}(t,S,T)
\right)^{2}
\bigg{|}\F_{t}
\right] 
\implies
a = \frac{
\int_{S}^{T}\E_{Q}[r(u)|\F_{t}]du
}{
(T-S)f^{3M}(t,S,T)
}
\end{align*}
\end{result} 

\newpage 

\subsection{Affine Term Structure-setting}

\begin{proposition}
Consider the above setting, and let $r = (r_{t})_{t\geq 0}$ be a model that provides ATS, then 
\begin{align*}
\argmin\limits_{a \in \R}&\E_{Q}\left[
\left(
X^{3M\_A}- af^{3M}(t,S,T)
\right)^{2}
\bigg{|}\F_{t}
\right] \\
&\Downarrow \\
a &= \frac{
r(t)(T-S)
+ \int_{S}^{T}\int_{t}^{u}b(s)dsdu 
+ \int_{S}^{T}\int_{t}^{u}\alpha(s)g(s)dsdu
}{
(T-S)f^{3M}(t,S,T)
}
\end{align*}
Where:
\begin{align*}
g(s) &= \exp\left(
\int_{t}^{s}\beta(v)dv
\right)
\left(
\int_{t}^{s}e^{-\int_{t}^{w}\beta(v)dv}b(w)dw + \E_{Q}[r(t)]
\right) 
\end{align*}
\end{proposition}

\begin{proof}
Consider the above setting, but now we assume that $r = (r_{t})_{t\geq 0}$ is a model that provides ATS (Affine Term Structure), now as described in proposition \ref{prop: condition_on_r_ATS}, we have that the dynamics of $r$ can be written as: 
\begin{align*}
dr(t) &= [b(t) + \beta(t)r(t)]dt + \sqrt{a(t) + \alpha(t)r(t)}dW^{Q}(t)
\end{align*}
Here $b, \beta, a, \alpha$ are deterministic continuous functions. Now from the dynamics, we get that for $u\geq t$: 
\begin{align*}
r(u) &= r(t) + \int_{t}^{u}b(s)ds + \int_{t}^{u}[\beta(s)r(s)]ds
+ \int_{t}^{u}\sqrt{\alpha(s)}dW^{Q}(s)
+ \int_{t}^{u}\sqrt{\alpha(s)r(s)}dW^{Q}(s)
\end{align*}

Each term is assumed to be Ito-integrable, i.e in $M^{2}([0,T])$, and by \\ $\F_{t}$-independence, we get:
\begin{align*}
\E_{Q}\left[
\int_{t}^{u}\sqrt{\alpha(s)}dW^{Q}(s)
\right]
&= 0 \\ 
\E_{Q}\left[
\int_{t}^{u}\sqrt{\alpha(s)r(s)}dW^{Q}(s)
\right] 
&= 0
\end{align*} 

And by using Stochastic-Fubini(\ref{thm: Stochastic_Fubini}), we get:
\begin{align*}
\E_{Q}\left[
\int_{t}^{u}[\beta(s)r(s)]ds
\right]
&= 
\int_{t}^{u}\beta(s)\E_{Q}[r(s)]ds
\end{align*}

This leaves us with: 
\begin{align*}
\int_{S}^{T}\E_{Q}[r(u)|\F_{t}]du 
&= r(t)(T-S)
+ \int_{S}^{T}\int_{t}^{u}b(s)dsdu 
+ \int_{S}^{T}\int_{t}^{u}\alpha(s)\E_{Q}[r(s)]dsdu
\end{align*}


\textbf{Overview of time-interval:}


\begin{tikzpicture}[snake=zigzag, line before snake = 5mm, line after snake = 5mm]
    % draw horizontal line   
    \draw (0,0) -- (9,0);
    %\draw[snake] (2,0) -- (4,0);
    %\draw (4,0) -- (5,0);
    %\draw[snake] (5,0) -- (7,0);
    %\draw[snake] (7,0) -- (9,0);
    %\draw (9,0) -- (10,0);

    % draw vertical lines
    \foreach \x in {0,2,4,5,7}
      \draw (\x cm,3pt) -- (\x cm,-3pt);

    % draw nodes
    \draw (0,0) node[below=3pt] {$ t $} node[above=3pt] {$   $};
    %\draw (1,0) node[below=3pt] {$ T_{0} $} node[above=3pt] {$  $};
    \draw (2,0) node[below=3pt] {$ S $} node[above=3pt] {$  $};
    %\draw (3,0) node[below=3pt] {$  $} node[above=3pt] {$  $};
    \draw (4,0) node[below=3pt] {$ s $} node[above=3pt] {$  $};
    \draw (5,0) node[below=3pt] {$ u $} node[above=3pt] {$  $};
    \draw (6,0) node[below=3pt] {$  $} node[above=3pt] {$  $};
    \draw (7,0) node[below=3pt] {$ T $} node[above=3pt] {$ $};
    %\draw (9,0) node[below=3pt] {$ T_{M} $} node[above=3pt] {$ $};
\end{tikzpicture} 
  
Thus in our setting we have: $t\leq S \leq s \leq u \leq T$, using same argument as above: 

\begin{align*}
r(s) &= r(t) + \int_{t}^{s}b(v)dv + \int_{t}^{s}[\beta(v)r(v)]dv
+ \int_{t}^{s}\sqrt{\alpha(v)}dW^{Q}(v)
+ \int_{t}^{s}\sqrt{\alpha(v)r(v)}dW^{Q}(v)    
\end{align*}

Now let $g(s) := \E_{Q}[r(s)]$: 
\begin{align*}
g(s) &= r(t) + \int_{t}^{s}b(v)dv + \int_{t}^{s}\beta(v)\E_{Q}[r(v)]dv
\end{align*}

Now taking the derivative w.r.t. $s$ and using the fundamental theorem of calculus, we get: 
\begin{align*}
g'(s) &= b(s) + \beta(s)\E_{Q}[r(s)] \\ 
&= b(s) + \beta(s)g(s), \; g(t) = \E_{Q}[r(t)]
\end{align*}

This is an ordinary differential equation, with the explicit solution given by:
\begin{align*}
 g(s) &= \exp\left(
 \int_{t}^{s}\beta(v)dv
 \right)
 \left(
 \int_{t}^{s}e^{-\int_{t}^{w}\beta(v)dv}b(w)dw + \E_{Q}[r(t)]
 \right)
\end{align*}
\end{proof}


\subsection{Hedging with available instruments in the market}

We now denote: 
\begin{align*}
X^{3M\_A} &= \frac{1}{T-S}\int_{S}^{T}r_{u}du = \frac{1}{T-S}Z \\ 
f^{3M\_A}(t,S,T) &= \frac{1}{T-S}\E_{Q}\left[
\int_{S}^{T}r_{u}du
\right] = \frac{1}{T-S}\E_{Q}[Z|\F_{t}]
\end{align*}

Now from Jensen's Inequality \ref{thm: Jensen's_ineuality}, we have that for $Z, \varphi(Z) \in L^{1}(\Omega, \F, Q)$, with $\varphi(x) = e^{x}$
\begin{align}
\label{eq: hedging_availible_inst_market_1}
\exp\left(
\E_{Q}[Z|\F_{t}]
\right)
&\leq 
\E_{Q}\left[
\exp(Z)|\F_{t}
\right] \nonumber \\ 
&\Updownarrow \nonumber \\ 
\exp\left(
(T-S)f^{3M\_A}(t,S,T)
\right) 
&\leq 
\E_{Q}\left[\exp(Z)|\F_{t}\right]
\end{align} 

Now from definition \ref{def: 3M_SOFR_futures}, we have: 
\begin{align}
\label{eq: hedging_availible_inst_market_2}
f^{3M}(t,S,T) &= \frac{1}{T-S}\left(
\E_{Q}\left[
\underbrace{e^{\int_{S}^{T}r_{u}du}}_{e^{Z}}
\bigg{|}\F_{t}\right] - 1
\right) \nonumber \\ 
&\Downarrow \nonumber \\ 
\E_{Q}[\exp(Z)|\F_{t}] &= (T-S)f^{3M}(t,S,T) + 1
\end{align}

Now by inserting \ref{eq: hedging_availible_inst_market_2} into \ref{eq: hedging_availible_inst_market_1} yields:

\begin{align*}
\exp\left(
(T-S)f^{3M\_A}(t,S,T)
\right) 
&\leq 
(T-S)f^{3M}(t,S,T) + 1 \\ 
&\Updownarrow \\
f^{3M\_A}(t,S,T) &\leq 
\frac{
\ln[(T-S)f^{3M}(t,S,T)]
}{
(T-S)
}
\end{align*}